cleaning, docs

Cslib/Languages/LambdaCalculus/LocallyNameless/Context.lean
@@ -17,43 +17,143 @@ Contexts as pairs of free variables and types.
 
 universe u v
 
-variable {Var : Type u} {Ty : Type v} [DecidableEq Var]
+variable {α : Type u} {β : Type v} [DecidableEq α]
+
+-- TODO: These are pieces of API that cannot be directly automated by adding `grind` attributes to
+-- `Mathlib.Data.List.Sigma`. We should consider upstreaming them to Mathlib.
+namespace List
+
+variable {β : α → Type v} {Γ Δ : List (Sigma β)}
+
+omit [DecidableEq α] in
+/-- Keys distribute with appending. -/
+theorem keys_append : (Δ ++ Γ).keys = Δ.keys ++ Γ.keys := by
+  induction Δ <;> simp_all
+
+/-- Sublists without duplicate keys preserve lookups. -/
+theorem sublist_dlookup (l₁ l₂ : List (Sigma β)) (nd₁ : l₁.NodupKeys) (nd₂ : l₂.NodupKeys)
+    (s : l₁ <+ l₂) (mem : b ∈ l₁.dlookup a) : b ∈ l₂.dlookup a := by
+  induction s generalizing a b
+  case slnil => exact mem
+  case cons p' _ ih =>
+    obtain ⟨a', b'⟩ := p'
+    have := ih nd₁ (by grind [nodupKeys_cons]) mem |> of_mem_dlookup |> mem_keys_of_mem
+    have : a ≠ a' := by grind [nodupKeys_cons]
+    simp_all
+  case cons₂ p' _ ih =>
+    obtain ⟨a', b'⟩ := p'
+    by_cases h : a = a'
+    · subst h
+      rw [List.dlookup_cons_eq] at *
+      exact mem
+    · simp_all
+
+/-- A lookup in appended lists must appear in one of the lists. -/
+theorem dlookup_append_mem (l₁ l₂ : List (Sigma β)) (mem : b ∈ (l₁ ++ l₂).dlookup a) : 
+    b ∈ l₁.dlookup a ∨ b ∈ l₂.dlookup a := by
+  rw [List.dlookup_append l₁ l₂ a] at mem
+  simp at mem
+  grind
+
+/-- List permutation preserves keys. -/
+theorem perm_keys (h : Γ.Perm Δ) : x ∈ Γ.keys ↔ x ∈ Δ.keys := by
+  induction h <;> grind [keys_cons]
+
+/-- A key not appearing in an appending of list must appear in either list. -/
+theorem nmem_append_keys (l₁ l₂ : List (Sigma β)) :
+    a ∉ (l₁ ++ l₂).keys ↔ a ∉ l₁.keys ∧ a ∉ l₂.keys := by
+  constructor <;> (
+    intro h
+    induction l₂
+    case nil => simp_all
+    case cons hd tl ih =>
+      have perm : (l₁ ++ hd :: tl).Perm (hd :: (l₁ ++ tl)) := by simp
+      grind [keys_cons, => perm_keys]
+  )
+
+end List
 
 namespace LambdaCalculus.LocallyNameless
 
 /-- A typing context is a list of free variables and corresponding types. -/
-abbrev Context (Var : Type u) (Ty : Type v) := List ((_ : Var) × Ty)
+abbrev Context (α : Type u) (β : Type v) := List ((_ : α) × β)
 
 namespace Context
 
 open List
 
+-- we would like grind to see through certain notations
+attribute [scoped grind =] Option.mem_def
+attribute [scoped grind _=_] List.append_eq
+attribute [scoped grind =] List.Nodup
+attribute [scoped grind =] List.NodupKeys
+attribute [scoped grind _=_] List.singleton_append
+
+-- a few grinds on Option:
+attribute [scoped grind =] Option.or_eq_some_iff
+attribute [scoped grind =] Option.or_eq_none_iff
+
+-- we would like grind to treat list and finset membership the same
+attribute [scoped grind _=_] List.mem_toFinset
+
+-- otherwise, we mostly reuse existing API in `Mathlib.Data.List.Sigma`
+attribute [scoped grind =] List.keys_cons
+attribute [scoped grind =] List.dlookup_cons_eq
+attribute [scoped grind =] List.dlookup_cons_ne
+attribute [scoped grind =] List.dlookup_nil
+attribute [scoped grind _=_] List.dlookup_isSome
+
 /-- The domain of a context is the finite set of free variables it uses. -/
 @[simp, grind =]
-def dom : Context Var Ty → Finset Var := toFinset ∘ keys
+def dom (Γ : Context α β) : Finset α := Γ.keys.toFinset
 
-/-- A well-formed context. -/
-abbrev Ok : Context Var Ty → Prop := NodupKeys
+instance : HasWellFormed (Context α β) :=
+  ⟨NodupKeys⟩
 
-instance : HasWellFormed (Context Var Ty) :=
-  ⟨Ok⟩
+omit [DecidableEq α] in
+@[scoped grind _=_]
+theorem haswellformed_def (Γ : Context α β) : Γ✓ = Γ.NodupKeys := by rfl
 
-variable {Γ Δ : Context Var Ty}
+variable {Γ Δ : Context α β}
 
 /-- Context membership is preserved on permuting a context. -/
-theorem dom_perm_mem_iff (h : Γ.Perm Δ) {x : Var} : x ∈ Γ.dom ↔ x ∈ Δ.dom := by
-  induction h <;> simp_all only [dom, Function.comp_apply, mem_toFinset, keys_cons, mem_cons] 
+theorem dom_perm_mem_iff (h : Γ.Perm Δ) {x : α} : x ∈ Γ.dom ↔ x ∈ Δ.dom := by
+  induction h <;> simp_all only [dom, mem_toFinset, keys_cons, mem_cons] 
   grind
 
-omit [DecidableEq Var] in
+omit [DecidableEq α] in
 /-- Context well-formedness is preserved on permuting a context. -/
 @[scoped grind →]
 theorem wf_perm (h : Γ.Perm Δ) : Γ✓ → Δ✓ := (List.perm_nodupKeys h).mp
 
-omit [DecidableEq Var] in
+omit [DecidableEq α] in
 /-- Context well-formedness is preserved on removing an element. -/
 @[scoped grind →]
 theorem wf_strengthen (ok : (Δ ++ ⟨x, σ⟩ :: Γ)✓) : (Δ ++ Γ)✓ := by
   exact List.NodupKeys.sublist (by simp) ok
+
+/-- A mapping of values within a context. -/
+@[simp, scoped grind]
+def map_val (f : β → β) (Γ : Context α β) : Context α β := 
+  Γ.map (fun ⟨var,ty⟩ => ⟨var,f ty⟩)
+
+omit [DecidableEq α] in
+/-- A mapping of values preserves keys. -/
+@[scoped grind]
+lemma map_val_keys (f) : Γ.keys = (Γ.map_val f).keys := by
+  induction Γ  <;> simp_all
+
+omit [DecidableEq α] in
+/-- A mapping of values preserves non-duplication of keys. -/
+theorem map_val_ok (f : β → β) : Γ✓ ↔ (Γ.map_val f)✓ := by
+  grind
+
+/-- A mapping of values maps lookups. -/
+lemma map_val_mem (mem : σ ∈ Γ.dlookup x) (f) : f σ ∈ (Γ.map_val f).dlookup x := by
+  induction Γ <;> grind
+
+/-- A mapping of values preserves non-lookups. -/
+lemma map_val_nmem (nmem : Γ.dlookup x = none) (f) : (Γ.map_val f).dlookup x = none := by
+  grind [List.dlookup_eq_none]
 
 end LambdaCalculus.LocallyNameless.Context
